got if's to step properly

CCode/fact.c
@@ -1,8 +1,8 @@
 int factorial(int n) {
 	int acc = 1;
 
-	for (int i = n; i > 0; --i) {
-		acc *= i;		
+	for (int i = 0; i < n; ++i) {
+		acc *= (n - i);		
 	}
 
 	return acc;
